verified/bitvectors.i.dfy
@@ -1,0 +1,178 @@
+include "bitvectors.s.dfy"
+include "ARMdef.dfy"
+
+lemma lemma_BitPos12()
+    ensures BitsAsWord(BitAtPos(12)) == 0x1000
+{
+    lemma_pow2_properties(12);
+}
+
+lemma lemma_BitOrOneIsLikePlus'(b: bv32)
+    requires BitMod(b, 2) == 0
+    ensures BitAdd(b, 1) == BitOr(b, 1)
+{
+    reveal_BitMod();
+    reveal_BitOr();
+    reveal_BitAdd();
+}
+
+lemma lemma_BitOrOneIsLikePlus(i: word)
+    requires i < 0xffffffff
+    requires i % 2 == 0
+    ensures i + 1 == BitwiseOr(i, 1)
+{
+    var b := WordAsBits(i);
+    reveal_WordAsBits();
+    reveal_BitsAsWord();
+    lemma_BitModEquiv(i, 2);
+    lemma_BitOrOneIsLikePlus'(b);
+    lemma_BitAddEquiv(i, 1);
+}
+
+lemma lemma_BitShift1(x: bv32)
+    requires x < 0x80000000
+    ensures BitShiftLeft(x, 1) == BitMul(x, 2)
+{
+    calc {
+        BitShiftLeft(x, 1);
+        { reveal_BitShiftLeft(); }
+        x << 1;
+        x * 2;
+        { reveal_BitMul(); }
+        BitMul(x, 2);
+    }
+}
+
+lemma lemma_LeftShift1(x: word)
+    requires x < 0x80000000
+    ensures LeftShift(x, 1) == x * 2
+{
+    calc {
+        LeftShift(x, 1);
+        BitsAsWord(BitShiftLeft(WordAsBits(x), 1));
+        { lemma_BitCmpEquiv(x, 0x80000000);
+          assert WordAsBits(0x80000000) == 0x80000000 by { reveal_WordAsBits(); }
+          lemma_BitShift1(WordAsBits(x)); }
+        BitsAsWord(BitMul(WordAsBits(x), 2));
+        { assert WordAsBits(2) == 2 by { reveal_WordAsBits(); } }
+        BitsAsWord(BitMul(WordAsBits(x), WordAsBits(2)));
+        { lemma_BitMulEquiv(x, 2); }
+        x * 2;
+    }
+}
+
+lemma lemma_LeftShiftsAdd(x: word, a: nat, b: nat)
+    requires 0 <= a + b < 32
+    ensures LeftShift(x, a + b) == LeftShift(LeftShift(x, a), b)
+{
+    calc {
+        LeftShift(x, a + b);
+        BitsAsWord(BitShiftLeft(WordAsBits(x), (a + b)));
+        { lemma_BitShiftsSum(WordAsBits(x), a, b); }
+        BitsAsWord(BitShiftLeft(BitShiftLeft(WordAsBits(x), a), b));
+        { lemma_BitsAsWordAsBits(BitShiftLeft(WordAsBits(x), a)); }
+        BitsAsWord(BitShiftLeft(WordAsBits(BitsAsWord(BitShiftLeft(WordAsBits(x), a))), b));
+        BitsAsWord(BitShiftLeft(WordAsBits(LeftShift(x, a)), b));
+        LeftShift(LeftShift(x, a), b);
+    }
+}
+
+lemma lemma_LeftShift2(x: word)
+    requires x < 0x40000000
+    ensures LeftShift(x, 2) == x * 4
+{
+    var x' := LeftShift(x, 1);
+    lemma_LeftShift1(x);
+    lemma_LeftShift1(x');
+    lemma_LeftShiftsAdd(x, 1, 1);
+}
+
+lemma lemma_LeftShift4(x: word)
+    requires x < 0x10000000
+    ensures LeftShift(x, 4) == x * 16
+{
+    var x' := LeftShift(x, 2);
+    lemma_LeftShift2(x);
+    lemma_LeftShift2(x');
+    lemma_LeftShiftsAdd(x, 2, 2);
+}
+
+lemma lemma_LeftShift12(x: word)
+    requires x < 0x100000
+    ensures LeftShift(x, 12) == x * 4096
+{
+    var x' := LeftShift(x, 4);
+    lemma_LeftShift4(x);
+    var x'' := LeftShift(x', 4);
+    lemma_LeftShift4(x');
+    lemma_LeftShiftsAdd(x, 4, 4);
+    assert x'' == LeftShift(x, 8);
+    assert x'' == x * 256;
+    var x''' := LeftShift(x'', 4);
+    lemma_LeftShift4(x'');
+    assert x''' == x * 4096;
+    lemma_LeftShiftsAdd(x, 8, 4);
+    assert x''' == LeftShift(x, 12);
+}
+
+function {:opaque} BitwiseMaskLow(i:word, bitpos:int): word
+    requires 0 <= bitpos < 32;
+    ensures BitwiseMaskLow(i, bitpos) == i % pow2(bitpos)
+    ensures pow2_properties(bitpos)
+{
+    lemma_BitmaskAsWord(i, bitpos);
+    lemma_pow2_properties(bitpos);
+    BitsAsWord(BitAnd(WordAsBits(i), BitmaskLow(bitpos)))
+}
+
+lemma lemma_Bitmask12()
+    ensures BitmaskLow(12) == 0xfff
+    ensures BitmaskHigh(12) == 0xfffff000
+{
+    calc {
+        BitmaskLow(12);
+        BitAtPos(12) - 1;
+        { lemma_BitsAsWordAsBits(BitAtPos(12)); }
+        WordAsBits(BitsAsWord(BitAtPos(12))) - 1;
+        WordAsBits(pow2(12)) - 1;
+        { lemma_pow2_properties(12); }
+        WordAsBits(0x1000) - 1;
+        { assert WordAsBits(0x1000) == 0x1000 by { reveal_WordAsBits(); }
+          lemma_BitSubEquiv(0x1000, 1); }
+        0xfff;
+    }
+
+    calc {
+        BitmaskHigh(12);
+        BitNot(BitmaskLow(12));
+        BitNot(0xfff);
+        { reveal_BitNot(); }
+        0xfffff000;
+    }
+}
+
+lemma lemma_Bitmask10()
+    ensures BitmaskLow(10) == 0x3ff
+    ensures BitmaskHigh(10) == 0xfffffc00
+{
+    calc {
+        BitmaskLow(10);
+        BitAtPos(10) - 1;
+        { lemma_BitsAsWordAsBits(BitAtPos(10)); }
+        WordAsBits(BitsAsWord(BitAtPos(10))) - 1;
+        WordAsBits(pow2(10)) - 1;
+        { lemma_pow2_properties(10); }
+        WordAsBits(0x400) - 1;
+        { assert WordAsBits(0x400) == 0x400 by { reveal_WordAsBits(); }
+          lemma_BitSubEquiv(0x400, 1); }
+        0x3ff;
+    }
+
+    calc {
+        BitmaskHigh(10);
+        BitNot(BitmaskLow(10));
+        BitNot(0x3ff);
+        { reveal_BitNot(); }
+        0xfffffc00;
+    }
+}
