verified/nlarith.s.dfy
@@ -7,3 +7,23 @@ lemma lemma_DivMulLessThan(a:int, b:int)
     requires b > 0
     ensures (a / b) * b <= a
 {}
+
+lemma lemma_DivBounds(a:int, b:int)
+    requires a >= 0 && b > 0
+    ensures 0 <= (a / b) <= a
+{
+    if a < b {
+        assert a / b == 0;
+    } else if a == b {
+        assert a / b == 1;
+    } else if b == 1 {
+        assert a / b == a;
+    } else if a > b {
+        assert 1 <= a / b < a;
+    }
+}
+
+lemma lemma_MulSign(a:int, b:int)
+    requires a >= 0 && b >= 0
+    ensures a * b >= 0
+{}
