verified/ptables.i.dfy
@@ -1,5 +1,6 @@
-include "pagedb.i.dfy"
 include "entry.s.dfy"
+include "pagedb.i.dfy"
+include "bitvectors.i.dfy"
 
 // XXX: this is placed at the top of the file to work around timeout
 // instability when verifying it later in the file
@@ -114,55 +115,274 @@ function mkAbsL1PTE(e: Maybe<PageNr>, subpage:int): Maybe<addr>
             Just(page_paddr(pgNr) + subpage * ARM_L2PTABLE_BYTES())
 }
 
-lemma {:axiom} lemma_l2ptesmatch(pte: L2PTE)
-    requires PhysBase() == KOM_DIRECTMAP_VBASE()
-    ensures ValidAbsL2PTEWord(mkL2Pte(pte)) && ExtractAbsL2PTE(mkL2Pte(pte)) == mkAbsPTE(pte)
-/* FIXME: this is really gross right now (and contains several
- * assumes!), largely due to problems in Boogie/Dafny's bitvector
- * support. It's also hopelessly unstable.
+lemma lemma_ARM_L2PTE(pa: word, w: bool, x: bool)
+    requires PageAligned(pa) && isUInt32(pa + PhysBase())
+    ensures ValidAbsL2PTEWord(ARM_L2PTE(pa, w, x))
+    ensures ExtractAbsL2PTE(ARM_L2PTE(pa, w, x)) == Just(AbsPTE(pa, w, x))
 {
-    var pteword := mkL2Pte(pte);
-    var ptebv := IntAsBits(pteword);
-    var extracted := ExtractAbsL2PTE(pteword);
+    lemma_Bitmask12();
+
+    var ptew := ARM_L2PTE(pa, w, x);
+    var nxbit:bv32 := if x then 0 else ARM_L2PTE_NX_BIT();
+    var robit:bv32 := if w then 0 else ARM_L2PTE_RO_BIT();
+    var extrabits := BitOr(BitOr(0xd76, nxbit), robit);
+    var pteb := BitOr(WordAsBits(pa), extrabits);
+
+    if x {
+        if w {
+            assert extrabits == 0xd76 by { reveal_BitOr(); }
+        } else {
+            assert extrabits == 0xf76 by { reveal_BitOr(); }
+        }
+    } else {
+        if w {
+            assert extrabits == 0xd77 by { reveal_BitOr(); }
+        } else {
+            assert extrabits == 0xf77 by { reveal_BitOr(); }
+        }
+    }
+
+    assert ptew == BitsAsWord(pteb) by {
+        calc {
+            ptew;
+            ARM_L2PTE(pa, w, x);
+            BitsAsWord(BitOr(WordAsBits(pa), BitOr(BitOr(ARM_L2PTE_CONST_BITS() | 0x2, nxbit), robit)));
+            { assert ARM_L2PTE_CONST_BITS() | 0x2 == 0xd76; }
+            BitsAsWord(BitOr(WordAsBits(pa), BitOr(BitOr(0xd76, nxbit), robit)));
+            BitsAsWord(BitOr(WordAsBits(pa), extrabits));
+        }
+    }
+    lemma_WordBitEquiv(ptew, pteb);
+
+    assert BitAnd(extrabits, 0xfffff000) == 0 by {
+        reveal_BitOr(); reveal_BitAnd();
+    }
+
+    assert BitAnd(WordAsBits(pa), 0xfff) == 0 by {
+        assert BitwiseMaskLow(pa, 12) == 0;
+        calc {
+            BitwiseMaskLow(pa, 12);
+            { reveal_BitwiseMaskLow(); }
+            BitsAsWord(BitAnd(WordAsBits(pa), BitmaskLow(12)));
+            BitsAsWord(BitAnd(WordAsBits(pa), 0xfff));
+        }
+    }
+
+    calc {
+        BitwiseMaskHigh(ptew, 12);
+        { reveal_BitwiseMaskHigh(); }
+        BitsAsWord(BitAnd(WordAsBits(ptew), BitmaskHigh(12)));
+        BitsAsWord(BitAnd(pteb, 0xfffff000));
+        BitsAsWord(BitAnd(BitOr(WordAsBits(pa), extrabits), 0xfffff000));
+        {
+            calc {
+                BitAnd(BitOr(WordAsBits(pa), extrabits), 0xfffff000);
+                { lemma_BitOrAndRelation(WordAsBits(pa), extrabits, 0xfffff000); }
+                BitOr(BitAnd(WordAsBits(pa), 0xfffff000), BitAnd(extrabits, 0xfffff000));
+                { assert BitAnd(extrabits, 0xfffff000) == 0 by { reveal_BitAnd(); } }
+                BitOr(BitAnd(WordAsBits(pa), 0xfffff000), 0);
+                { reveal_BitOr(); }
+                BitAnd(WordAsBits(pa), 0xfffff000);
+                { assert BitAnd(WordAsBits(pa), 0xfff) == 0; reveal_BitAnd(); }
+                WordAsBits(pa);
+            }
+        }
+        BitsAsWord(WordAsBits(pa));
+        { lemma_WordAsBitsAsWord(pa); }
+        pa;
+    }
+    assert BitwiseMaskHigh(ptew, 12) == pa;
+
+    assert BitAnd(pteb, 0x3) == 2 || BitAnd(pteb, 0x3) == 3 by {
+        calc {
+            BitAnd(pteb, 0x3);
+            BitAnd(BitOr(WordAsBits(pa), extrabits), 0x3);
+            { lemma_BitOrAndRelation(WordAsBits(pa), extrabits, 0x3); }
+            BitOr(BitAnd(WordAsBits(pa), 0x3), BitAnd(extrabits, 0x3));
+            { calc {
+                BitAnd(WordAsBits(pa), 0x3);
+                { assert BitAnd(WordAsBits(pa), 0xfff) == 0; reveal_BitAnd(); }
+                0;
+            } }
+            BitOr(0, BitAnd(extrabits, 0x3));
+            { reveal_BitOr(); }
+            BitAnd(extrabits, 0x3);
+        }
+        reveal_BitAnd();
+    }
+
+    assert BitAnd(pteb, 0xdfc) == ARM_L2PTE_CONST_BITS() by {
+        calc {
+            BitAnd(pteb, 0xdfc);
+            BitAnd(BitOr(WordAsBits(pa), extrabits), 0xdfc);
+            { lemma_BitOrAndRelation(WordAsBits(pa), extrabits, 0xdfc); }
+            BitOr(BitAnd(WordAsBits(pa), 0xdfc), BitAnd(extrabits, 0xdfc));
+            { calc {
+                BitAnd(WordAsBits(pa), 0xdfc);
+                { assert BitAnd(WordAsBits(pa), 0xfff) == 0; reveal_BitAnd(); }
+                0;
+            } }
+            BitOr(0, BitAnd(extrabits, 0xdfc));
+            { reveal_BitOr(); }
+            BitAnd(extrabits, 0xdfc);
+            { reveal_BitAnd(); }
+            0xd74;
+            ARM_L2PTE_CONST_BITS();
+        }
+    }
+
+    assert x == (BitAnd(pteb, ARM_L2PTE_NX_BIT()) == 0) by {
+        calc {
+            BitAnd(pteb, ARM_L2PTE_NX_BIT());
+            BitAnd(BitOr(WordAsBits(pa), extrabits), 1);
+            { lemma_BitOrAndRelation(WordAsBits(pa), extrabits, 1); }
+            BitOr(BitAnd(WordAsBits(pa), 1), BitAnd(extrabits, 1));
+            { calc {
+                BitAnd(WordAsBits(pa), 1);
+                { assert BitAnd(WordAsBits(pa), 0xfff) == 0; reveal_BitAnd(); }
+                0;
+            } }
+            BitOr(0, BitAnd(extrabits, 1));
+            { reveal_BitOr(); }
+            BitAnd(extrabits, 1);
+            { reveal_BitAnd(); }
+            nxbit;
+        }
+    }
+
+    assert w == (BitAnd(pteb, ARM_L2PTE_RO_BIT()) == 0) by {
+        calc {
+            BitAnd(pteb, ARM_L2PTE_RO_BIT());
+            BitAnd(BitOr(WordAsBits(pa), extrabits), 0x200);
+            { lemma_BitOrAndRelation(WordAsBits(pa), extrabits, 0x200); }
+            BitOr(BitAnd(WordAsBits(pa), 0x200), BitAnd(extrabits, 0x200));
+            { calc {
+                BitAnd(WordAsBits(pa), 0x200);
+                { assert BitAnd(WordAsBits(pa), 0xfff) == 0; reveal_BitAnd(); }
+                0;
+            } }
+            BitOr(0, BitAnd(extrabits, 0x200));
+            { reveal_BitOr(); }
+            BitAnd(extrabits, 0x200);
+            { reveal_BitAnd(); }
+            robit;
+        }
+    }
+}
+
+lemma lemma_l2ptesmatch(pte: L2PTE)
+    requires PhysBase() == KOM_DIRECTMAP_VBASE()
+    ensures ValidAbsL2PTEWord(mkL2Pte(pte))
+    ensures ExtractAbsL2PTE(mkL2Pte(pte)) == mkAbsPTE(pte)
+{
+    lemma_Bitmask12();
+
+    var ptew := mkL2Pte(pte);
+    var pteb := WordAsBits(ptew);
+    lemma_WordBitEquiv(ptew, pteb);
+    var extracted := if ValidAbsL2PTEWord(ptew) then Just(ExtractAbsL2PTE(ptew)) else Nothing;
+
     if pte.NoMapping? {
-        assert ptebv == 0;
-        assert extracted == Just(Nothing) by {reveal_BitAnd();}
+        assert pteb == 0;
+        assert BitAnd(pteb, 0x3) == 0 by { reveal_BitAnd(); }
+        assert extracted == Just(Nothing);
     } else {
         var pa, w, x;
         match pte {
             case SecureMapping(p, ws, xs) =>
                 pa, w, x := page_paddr(p), ws, xs;
             case InsecureMapping(p, wi) =>
+                assert validInsecurePageNr(p);
                 pa, w, x := p * PAGESIZE(), wi, false;
         }
-        assert pteword == ARM_L2PTE(pa, w, x);
-        var pabv := IntAsBits(pa);
-        assert PAGESIZE() == 0x1000 == pow2(12) by { reveal_pow2(); }
-        assert pa % PAGESIZE() == 0;
-        assert BitmaskLow(12) == 0xfff by { reveal_BitmaskLow(); assume 1 as bv32 << 12 == 0x1000; }
-        reveal_BitAnd();
-        assert BitAnd(pabv, 0xfff) == 0 by { lemma_Bitmask(pabv, 12); lemma_BitModEquiv(pabv, 0x1000); }
-        var nxbit:bv32 := if x then 0 else ARM_L2PTE_NX_BIT();
-        var robit:bv32 := if w then 0 else ARM_L2PTE_RO_BIT();
-        assert ARM_L2PTE_NX_BIT() == 1 && ARM_L2PTE_RO_BIT() == 0x200;
-        assert ptebv == pabv | ARM_L2PTE_CONST_BITS() | 0x2 | nxbit | robit;
-        assert BitAnd(ptebv, 0x3) == 2;
-        assert BitAnd(ptebv, 0xfdfc) == ARM_L2PTE_CONST_BITS();
-        assert BitAnd(ptebv, 0xfffff000) == IntAsBits(pa);
-        assert pa == BitwiseMaskHigh(pteword, 12) by { reveal_BitmaskHigh(); reveal_BitNot(); assume 1 as bv32 << 12 == 0x1000; }
-        assert ptebv & ARM_L2PTE_NX_BIT() == nxbit;
-        assert ptebv & ARM_L2PTE_RO_BIT() == robit;
+        assert ptew == ARM_L2PTE(pa, w, x);
+        lemma_ARM_L2PTE(pa, w, x);
         assert isUInt32(pa + PhysBase());
         assert extracted == Just(mkAbsPTE(pte));
     }
-} */
+}
 
-lemma {:axiom} lemma_l1ptesmatch(e: Maybe<PageNr>, subpage:int)
+lemma lemma_l1ptesmatch(e: Maybe<PageNr>, subpage:int)
     requires 0 <= subpage < 4
     requires PhysBase() == KOM_DIRECTMAP_VBASE()
     ensures ValidAbsL1PTEWord(mkL1Pte(e, subpage))
     ensures ExtractAbsL1PTE(mkL1Pte(e, subpage)) == mkAbsL1PTE(e, subpage)
-    /* TODO: as above */
+{
+    var ptew := mkL1Pte(e, subpage);
+    var pteb := WordAsBits(ptew);
+    lemma_WordBitEquiv(ptew, pteb);
+
+    assert WordAsBits(0x3fc) == 0x3fc && WordAsBits(0x3) == 0x3
+        && WordAsBits(1) == 1 by { reveal_WordAsBits(); }
+
+    match e {
+    case Nothing => assert ptew == 0; reveal_BitAnd();
+    case Just(pg) => {
+        var pa := page_paddr(pg) + subpage * ARM_L2PTABLE_BYTES();
+        assert pa % ARM_L2PTABLE_BYTES() == 0;
+        assert ptew == ARM_L1PTE(pa);
+
+        calc {
+            1;
+            { lemma_BitOrOneIsLikePlus(pa); }
+            BitwiseMaskLow(ptew, 10);
+            { reveal_BitwiseMaskLow(); }
+            BitsAsWord(BitAnd(WordAsBits(ptew), BitmaskLow(10)));
+            { lemma_Bitmask10(); }
+            BitsAsWord(BitAnd(WordAsBits(ptew), 0x3ff));
+            BitsAsWord(BitAnd(pteb, 0x3ff));
+        }
+        calc {
+            1;
+            WordAsBits(BitsAsWord(BitAnd(pteb, 0x3ff)));
+            { lemma_BitsAsWordAsBits(BitAnd(pteb, 0x3ff)); }
+            BitAnd(pteb, 0x3ff);
+        }
+
+        assert BitwiseAnd(ptew, 0x3) == 1 && BitwiseAnd(ptew, 0x3fc) == 0 by {
+            assert BitAnd(pteb, 0x3) == 1 && BitAnd(pteb, 0x3fc) == 0 by {
+                reveal_BitAnd();
+            }
+        }
+
+        calc {
+            BitwiseMaskHigh(ptew, 10);
+            { reveal_BitwiseMaskHigh(); }
+            BitsAsWord(BitAnd(WordAsBits(ptew), BitmaskHigh(10)));
+            { calc {
+                BitAnd(WordAsBits(ptew), BitmaskHigh(10));
+                { lemma_Bitmask10(); }
+                BitAnd(pteb, 0xfffffc00);
+                BitAnd(WordAsBits(ARM_L1PTE(pa)), 0xfffffc00);
+                BitAnd(WordAsBits(BitwiseOr(pa, 1)), 0xfffffc00);
+                BitAnd(WordAsBits(BitsAsWord(BitOr(WordAsBits(pa), WordAsBits(1)))),
+                    0xfffffc00);
+                { lemma_BitsAsWordAsBits(BitOr(WordAsBits(pa), WordAsBits(1)));
+                  assert WordAsBits(1) == 1 by { reveal_WordAsBits(); } }
+                BitAnd(BitOr(WordAsBits(pa), 1), 0xfffffc00);
+                BitAnd(BitOr(WordAsBits(pa), 1), 0xfffffc00);
+                { lemma_BitOrAndRelation(WordAsBits(pa), 1, 0xfffffc00); }
+                BitOr(BitAnd(WordAsBits(pa), 0xfffffc00), BitAnd(1, 0xfffffc00));
+                { reveal_BitAnd(); }
+                BitOr(BitAnd(WordAsBits(pa), 0xfffffc00), 0);
+                { reveal_BitOr(); }
+                BitAnd(WordAsBits(pa), 0xfffffc00);
+                { calc {
+                    0;
+                    BitwiseMaskLow(pa, 10);
+                    { reveal_BitwiseMaskLow(); }
+                    BitsAsWord(BitAnd(WordAsBits(pa), BitmaskLow(10)));
+                    { lemma_Bitmask10(); }
+                    BitsAsWord(BitAnd(WordAsBits(pa), 0x3ff));
+                } assert BitAnd(WordAsBits(pa), 0x3ff) == 0; reveal_BitAnd(); }
+                WordAsBits(pa);
+            } }
+            BitsAsWord(WordAsBits(pa));
+            { lemma_WordAsBitsAsWord(pa); }
+            pa;
+        }
+    } }
+}
 
 function mkAbsL2PTable(e:PageDbEntryTyped, i:int): AbsL2PTable
     requires PhysBase() == KOM_DIRECTMAP_VBASE()
